src/mapping/PStoRMWConsistent.v
@@ -93,7 +93,7 @@ Module PStoRMWConsistent.
                exists fts fval ftid,
                  (<<FROM: from = ntt fts>>) /\
                  (<<GET_FROM_ARM: Memory.get_msg fts mem_arm = Some (Msg.mk msg_arm.(Msg.loc) fval ftid)>>) /\
-                 (<<LATEST: Memory.latest msg_arm.(Msg.loc) fts ts mem_arm>>))) /\
+                 (<<EMPTY: empty_loc msg_arm.(Msg.loc) fts ts mem_arm>>))) /\
             (__guard__ (
                (<<MSG: msg_ps = Message.reserve>>) /\
                (<<PROMISED_ARM: Promises.lookup ts lc_arm.(Local.promises) <-> msg_arm.(Msg.tid) = tid>>) /\
@@ -1307,7 +1307,7 @@ Module PStoRMWConsistent.
         (TS: told < tnew)
         (OLD: Memory.read loc told mem_arm = Some vold)
         (NEW: Memory.get_msg tnew mem_arm = Some msg)
-        (EX: ex_strong loc told tnew mem_arm)
+        (EX: empty_loc loc told tnew mem_arm)
         (LOC1: msg.(Msg.loc) = loc)
         (LOC2: loc = Zpos loc_ps)
         (RESERVED: PSMemory.get loc_ps (ntt tnew) mem_ps = Some (from, Message.reserve)):
@@ -1339,7 +1339,7 @@ Module PStoRMWConsistent.
       }
       inv l; ss. exfalso.
       unfold Memory.read in OLD. ss. des_ifs.
-      exploit LATEST; try exact Heq; ss; try nia.
+      exploit EMPTY; try exact Heq; ss; try nia.
     }
   Qed.
 
@@ -1778,7 +1778,7 @@ Module PStoRMWConsistent.
           { instantiate (1:=Msg.mk vloc.(ValA.val) vnew.(ValA.val) tid).
             inv STEP_FULFILL. ss.
           }
-          { hexploit update_ex_strong; try exact STEP_READ; try exact STEP_FULFILL; ss.
+          { hexploit update_empty_loc; try exact STEP_READ; try exact STEP_FULFILL; ss.
             eapply RMWLocal.control_fulfillable; eauto.
           }
           { ss. }
