src/mapping/PStoRMWInit.v
@@ -1,0 +1,252 @@
+Require Import NArith.
+Require Import PArith.
+Require Import ZArith.
+Require Import Lia.
+Require Import EquivDec.
+Require Import RelationClasses.
+Require Import Bool.
+
+From sflib Require Import sflib.
+From Paco Require Import paco.
+
+From PromisingLib Require Import Basic.
+From PromisingLib Require Import Axioms.
+From PromisingLib Require Import Language.
+From PromisingLib Require Import Event.
+From PromisingLib Require Import Loc.
+
+From PromisingIR Require Import Time.
+From PromisingIR Require Import View.
+From PromisingIR Require Import BoolMap.
+From PromisingIR Require Import Promises.
+From PromisingIR Require Import Cell.
+From PromisingIR Require Import Memory.
+From PromisingIR Require Import TView.
+From PromisingIR Require Import Global.
+From PromisingIR Require Import Local.
+From PromisingIR Require Import Thread.
+From PromisingIR Require Import Configuration.
+
+Require Import PromisingArch.lib.Basic.
+Require Import PromisingArch.lib.Order.
+Require Import PromisingArch.lib.Time.
+Require Import PromisingArch.lib.Lang.
+
+Require Import PromisingArch.promising.Promising.
+Require Import PromisingArch.mapping.RMWLang.
+Require Import PromisingArch.mapping.RMWPromising.
+Require Import PromisingArch.mapping.PSLang.
+Require Import PromisingArch.mapping.PStoRMWUtils.
+Require Import PromisingArch.mapping.PStoRMWDef.
+Require Import PromisingArch.mapping.PStoRMWThread.
+Require Import PromisingArch.mapping.PStoRMWConsistent.
+
+Set Implicit Arguments.
+Set Nested Proofs Allowed.
+
+
+Module PStoRMWInit.
+  Import PStoRMWThread.
+
+  Variant sim_memory_init (tid: Ident.t) (rsv_ps: PSMemory.t) (mem_ps: PSMemory.t) (mem_arm: Memory.t): Prop :=
+    | sim_memory_init_intro
+        (MEM_SOUND: forall ts msg_arm
+                           (GET_ARM: Memory.get_msg ts mem_arm = Some msg_arm),
+          exists loc_ps from,
+            (<<LOC: msg_arm.(Msg.loc) = Zpos loc_ps>>) /\
+            (<<GET_PS: PSMemory.get loc_ps (ntt ts) mem_ps = Some (from, Message.reserve)>>) /\
+            (<<RESERVED: msg_arm.(Msg.tid) = tid ->
+                         PSMemory.get loc_ps (ntt ts) rsv_ps = Some (from, Message.reserve)>>) /\
+            (<<TS: PSTime.lt from (ntt ts)>>) /\
+            (__guard__ (
+               (<<FROM: from = PSTime.bot>>) \/
+               exists fts fval ftid,
+                 (<<FROM: from = ntt fts>>) /\
+                 (<<GET_FROM_ARM: Memory.get_msg fts mem_arm = Some (Msg.mk msg_arm.(Msg.loc) fval ftid)>>) /\
+                 (<<EMPTY: empty_loc msg_arm.(Msg.loc) fts ts mem_arm>>))))
+        (MEM_COMPLETE: forall loc_ps from to msg_ps
+                              (TO: PSTime.lt PSTime.bot to)
+                              (GET_PS: PSMemory.get loc_ps to mem_ps = Some (from, msg_ps)),
+          exists ts msg_arm,
+            (<<TO: to = ntt ts>>) /\
+            (<<MSG_PS: msg_ps = Message.reserve>>) /\
+            (<<GET_ARM: Memory.get_msg ts mem_arm = Some msg_arm>>) /\
+            (<<LOC: msg_arm.(Msg.loc) = Zpos loc_ps>>))
+  .
+
+  Variant sim_thread_init (tid: Ident.t) (th_ps: PSThread.t lang_ps) (eu: RMWExecUnit.t (A:=unit)): Prop :=
+    | sim_thread_init_intro
+        (SIM_MEM: sim_memory_init tid
+                                  (PSLocal.reserves (PSThread.local th_ps))
+                                  (PSGlobal.memory (PSThread.global th_ps))
+                                  (RMWExecUnit.mem eu))
+  .
+
+  Definition ps_locations_only (mem: Memory.t): Prop :=
+    forall ts msg_arm (GET: Memory.get_msg ts mem = Some msg_arm),
+    exists loc_ps, msg_arm.(Msg.loc) = Zpos loc_ps.
+
+  Lemma promise_step_ps_locations_only
+        tid (eu1 eu2: RMWExecUnit.t (A:=unit))
+        (LOCS: ps_locations_only eu2.(RMWExecUnit.mem))
+        (STEP: RMWExecUnit.promise_step tid eu1 eu2):
+    ps_locations_only eu1.(RMWExecUnit.mem).
+  Proof.
+    destruct eu1, eu2.
+    inv STEP. inv LOCAL. inv MEM2. ss. subst.
+    ii. unfold Memory.get_msg in GET.
+    destruct ts; ss.
+    exploit (LOCS (S ts)).
+    { unfold Memory.get_msg. s.
+      eapply nth_error_app_mon; eauto.
+    }
+    i. des. eauto.
+  Qed.
+
+  Lemma init_sim_memory_init tid:
+    sim_memory_init tid PSMemory.bot PSMemory.init Memory.empty.
+  Proof.
+    econs; i.
+    - unfold Memory.get_msg in *. destruct ts; ss.
+      apply nth_error_some in GET_ARM. ss. nia.
+    - exploit PSMemory.init_get; eauto. i. des. subst. inv TO.
+  Qed.
+
+  Lemma empty_loc_app
+        loc from to mem1 mem2
+        (TO: to <= S (length mem1))
+        (EMPTY: empty_loc loc from to mem1):
+    empty_loc loc from to (mem1 ++ mem2).
+  Proof.
+    ii. eapply EMPTY; eauto.
+    rewrite List.nth_error_app1 in MSG; ss. nia.
+  Qed.
+
+  Lemma read_ts
+        loc ts mem val
+        (READ: Memory.read loc ts mem = Some val):
+    ts <= length mem.
+  Proof.
+    unfold Memory.read in *.
+    destruct ts; ss; try nia. des_ifs.
+    exploit nth_error_some; eauto.
+  Qed.
+
+  Lemma get_msg_ts
+        ts mem msg
+        (GET: Memory.get_msg ts mem = Some msg):
+    ts <= length mem.
+  Proof.
+    unfold Memory.get_msg in *.
+    destruct ts; ss.
+    exploit nth_error_some; eauto.
+  Qed.
+
+  Lemma incr_ntt_S ts: PSTime.incr (ntt ts) = ntt (S ts).
+  Proof.
+    ss.
+  Qed.
+
+  Lemma sim_memory_init_promise_step
+        tid th1_ps (eu1 eu2: RMWExecUnit.t (A:=unit))
+        (SIM1: sim_thread_init tid th1_ps eu1)
+        (LC_WF1_PS: PSLocal.wf (PSThread.local th1_ps) (PSThread.global th1_ps))
+        (LOCS: ps_locations_only eu2.(RMWExecUnit.mem))
+        (STEP: RMWExecUnit.promise_step tid eu1 eu2):
+    exists loc from to th2_ps,
+      (<<STEP_PS: PSThread.step (ThreadEvent.reserve loc from to) th1_ps th2_ps>>) /\
+      (<<SIM2: sim_thread_init tid th2_ps eu2>>).
+  Proof.
+    destruct th1_ps as [st1_ps lc1_ps [sc1_ps gprm1_ps mem1_ps]].
+    destruct eu1 as [st1_arm lc1_arm mem1_arm].
+    destruct eu2 as [st2_arm lc2_arm mem2_arm].
+    inv SIM1. ss. inv STEP. ss. subst.
+    inv LOCAL. inv MEM2.
+    exploit (LOCS (S (length mem1_arm))).
+    { unfold Memory.get_msg. ss.
+      rewrite List.nth_error_app2; try refl.
+      rewrite Nat.sub_diag. ss.
+    }
+    s. i. des. subst.
+    specialize (Memory.get_latest (Zpos loc_ps) mem1_arm). i. des.
+    exploit (@PSMemory.add_exists mem1_ps loc_ps (ntt ts) (ntt (S (length mem1_arm))) Message.reserve).
+    { i. inv SIM_MEM.
+      destruct (TimeFacts.le_lt_dec to2 PSTime.bot).
+      { ii. inv LHS. inv RHS. ss.
+        cut (PSTime.lt from2 PSTime.bot).
+        { i. inv H1. }
+        eapply TimeFacts.lt_le_lt; eauto.
+      }
+      exploit MEM_COMPLETE; eauto. i. des. subst.
+      unfold Memory.get_msg in GET_ARM. destruct ts0; ss.
+      exploit (H (S ts0)).
+      { unfold Memory.read. ss. rewrite GET_ARM.
+        rewrite LOC. condtac; ss. congr.
+      }
+      ii. inv LHS. inv RHS. ss.
+      exploit TimeFacts.lt_le_lt; [exact FROM|exact TO0|]. i.
+      rewrite incr_ntt_S in *.
+      apply ntt_lt in x2. nia.
+    }
+    { apply lt_ntt.
+      exploit Memory.read_get_msg; eauto. i. des.
+      { subst. unfold Time.bot. nia. }
+      unfold Memory.get_msg in *. destruct ts; ss.
+      exploit nth_error_some; eauto. i. nia.
+    }
+    { econs. }
+    i. des.
+    exploit PSMemory.add_exists_le; try exact x0; try apply LC_WF1_PS. i. des.
+
+    esplits.
+    { econs 1. econs 2. econs; eauto. }
+    { inv SIM_MEM. econs. ss. econs; i.
+      { exploit Memory.get_msg_snoc_inv; eauto. i. des.
+        - exploit MEM_SOUND; eauto. i. des.
+          exploit PSMemory.add_get1; try exact GET_PS; eauto. i.
+          esplits; eauto.
+          + i. exploit RESERVED; eauto. i.
+            eapply PSMemory.add_get1; eauto.
+          + unguard. des; eauto. right. subst.
+            exploit Memory.get_msg_mon; try exact GET_FROM_ARM. i.
+            esplits; eauto.
+            eapply empty_loc_app; eauto.
+        - subst.
+          exploit PSMemory.add_get0; try exact x0. i. des.
+          exploit PSMemory.add_get0; try exact x1. i. des.
+          esplits; ss; eauto.
+          + rewrite incr_ntt_S. apply lt_ntt.
+            exploit read_ts; try exact H0. i. nia.
+          + unguard. destruct ts; auto. right.
+            unfold Memory.read in H0. ss. des_ifs.
+            destruct t. ss. r in e. subst.
+            esplits.
+            * rewrite incr_ntt_S. refl.
+            * unfold Memory.get_msg. ss.
+              eapply nth_error_app_mon; eauto.
+            * ii. rewrite List.nth_error_app1 in MSG; try nia.
+              exploit (H (S ts0)).
+              { unfold Memory.read. s.
+                rewrite MSG, LOC. condtac; ss. congr.
+              }
+              i. nia.
+      }
+      { revert GET_PS.
+        erewrite PSMemory.add_o; eauto. condtac; ss; i.
+        - des. inv GET_PS. esplits.
+          + rewrite incr_ntt_S. refl.
+          + ss.
+          + unfold Memory.get_msg. s.
+            rewrite List.nth_error_app2; try refl.
+            rewrite Nat.sub_diag. ss.
+          + ss.
+        - guardH o.
+          exploit MEM_COMPLETE; eauto. i. des.
+          esplits; eauto.
+          revert GET_ARM. unfold Memory.get_msg.
+          destruct ts0; ss. i.
+          eapply nth_error_app_mon; eauto.
+      }
+    }
+  Qed.    
+End PStoRMWInit.
